First let us denote by $t$ the index in which $y$ has the 1. For simplicity, we assume that the base of the log is $e$.
We get that 
$$CE(\hat{y})= -\sum_i y_i log(\hat{y}_i)=-log(\hat{y}_t)=-log(\frac{exp(\theta_t)}{\sum_j exp(\theta_j)})=-\theta_t + log(\sum_j exp(\theta_j))$$
Let us look at the right term of the last equation. We get that $$\frac{\partial log(\sum_j exp(\theta_j))}{\partial \theta_i}=\frac{exp(\theta_i)}{\sum_j exp(\theta_j)}=\hat{y}_i$$
For the term we that $\frac{\partial -\theta_t}{\partial \theta_i}=-1$ if $i=t$ and $0$ otherwise. To summarize, we get 
$$
\frac{\partial CE}{\partial \theta_i}=
\begin{cases}
\hat{y}_i - 1, \text{ } i=t  \\ 
\hat{y}_i, \text{     } i\neq t
\end{cases} = \hat{y}-y
$$
Note that the partial derivative for $\theta_t$ is negative, which makes sense since when applying SGD we subtract the derivative from the current value of $\theta_t$, hence we would enlarge $\theta_t$ and minimize the loss. For all other $i \neq t$ the derivative is positive.